compiler/bytecode/miscScript.sml
@@ -4,6 +4,58 @@ val _ = new_theory "misc"
 
 (* TODO: move/categorize *)
 
+val ALOOKUP_APPEND_same = store_thm("ALOOKUP_APPEND_same",
+  ``∀l1 l2 l. (ALOOKUP l1 = ALOOKUP l2) ==> (ALOOKUP (l1 ++ l) = ALOOKUP (l2 ++ l))``,
+  rw[ALOOKUP_APPEND,FUN_EQ_THM])
+
+val ALOOKUP_ALL_DISTINCT_PERM_same = store_thm("ALOOKUP_ALL_DISTINCT_PERM_same",
+  ``∀l1 l2. ALL_DISTINCT (MAP FST l1) ∧ PERM (MAP FST l1) (MAP FST l2) ∧ (set l1 = set l2) ⇒ (ALOOKUP l1 = ALOOKUP l2)``,
+  simp[EXTENSION] >>
+  rw[FUN_EQ_THM] >>
+  Cases_on`ALOOKUP l2 x` >- (
+    imp_res_tac ALOOKUP_FAILS >>
+    imp_res_tac MEM_PERM >>
+    fs[FORALL_PROD,MEM_MAP,EXISTS_PROD] >>
+    metis_tac[ALOOKUP_FAILS] ) >>
+  qmatch_assum_rename_tac`ALOOKUP l2 x = SOME p`[] >>
+  imp_res_tac ALOOKUP_MEM >>
+  `ALL_DISTINCT (MAP FST l2)` by (
+    metis_tac[ALL_DISTINCT_PERM]) >>
+  imp_res_tac ALOOKUP_ALL_DISTINCT_MEM >>
+  metis_tac[])
+
+val ALL_DISTINCT_PERM_ALOOKUP_ZIP = store_thm("ALL_DISTINCT_PERM_ALOOKUP_ZIP",
+  ``∀l1 l2 l3. ALL_DISTINCT (MAP FST l1) ∧ PERM (MAP FST l1) l2
+    ⇒ (set l1 = set (ZIP (l2, MAP (THE o ALOOKUP (l1 ++ l3)) l2)))``,
+  rw[EXTENSION,FORALL_PROD,EQ_IMP_THM] >- (
+    qmatch_assum_rename_tac`MEM (x,y) l1`[] >>
+    imp_res_tac PERM_LENGTH >> fs[] >>
+    simp[MEM_ZIP] >>
+    imp_res_tac MEM_PERM >>
+    fs[MEM_MAP,EXISTS_PROD] >>
+    `MEM x l2` by metis_tac[] >>
+    `∃m. m < LENGTH l2 ∧ (x = EL m l2)` by metis_tac[MEM_EL] >>
+    qexists_tac`m`>>simp[]>>
+    simp[EL_MAP] >>
+    imp_res_tac ALOOKUP_ALL_DISTINCT_MEM >>
+    rw[ALOOKUP_APPEND] ) >>
+  qmatch_rename_tac`MEM (x,y) l1`[] >>
+  imp_res_tac PERM_LENGTH >>
+  fs[MEM_ZIP] >>
+  simp[EL_MAP] >>
+  imp_res_tac MEM_PERM >>
+  fs[MEM_EL,GSYM LEFT_FORALL_IMP_THM] >>
+  first_x_assum(qspec_then`n`mp_tac) >>
+  discharge_hyps >- simp[] >>
+  disch_then(Q.X_CHOOSE_THEN`m`strip_assume_tac) >>
+  qexists_tac`m` >>
+  simp[EL_MAP] >>
+  Cases_on`EL m l1`>>simp[ALOOKUP_APPEND] >>
+  BasicProvers.CASE_TAC >- (
+    imp_res_tac ALOOKUP_FAILS >>
+    metis_tac[MEM_EL] ) >>
+  metis_tac[MEM_EL,ALOOKUP_ALL_DISTINCT_MEM,optionTheory.THE_DEF])
+
 val PERM_ZIP = store_thm("PERM_ZIP",
   ``∀l1 l2. PERM l1 l2 ⇒ ∀a b c d. (l1 = ZIP(a,b)) ∧ (l2 = ZIP(c,d)) ∧ (LENGTH a = LENGTH b) ∧ (LENGTH c = LENGTH d) ⇒
     PERM a c ∧ PERM b d``,
